better cfg rendering

src/Analysis/Instances/Tooling/Analysis_GraphViz.thy
@@ -561,5 +561,430 @@ definition ctx_annotated_graphviz ::
        @ concat (map (ctx_annot_cluster vid nlab ckey clabel ns es) ks)
        @ ''}'' @ [CHR 0x0A]"
 
+section \<open>Generic context-expanded analysis graph\<close>
+
+text \<open>
+  The analysis graph is independent of DOT.  It records contextual local nodes,
+  shared global nodes, and the semantic role of every routed edge.  The builder
+  consumes the same routing function as the equation generator; it never
+  reconstructs contexts from labels or example-specific values.
+\<close>
+
+datatype ('ctx, 'g) analysis_cluster =
+    ContextCluster string 'ctx
+  | GlobalCluster
+
+datatype ('ctx, 'g) analysis_node =
+    LocalNode pp 'ctx
+  | GlobalNode 'g
+
+datatype analysis_edge_kind =
+    IntraEdge edge_action
+  | EnterEdge edge_action
+  | CombineEdge pp "vname option" "vname option"
+  | GlobalReadEdge
+  | GlobalWriteEdge
+
+type_synonym ('ctx, 'g) analysis_graph =
+  "(('ctx, 'g) analysis_cluster list \<times>
+    ('ctx, 'g) analysis_node list \<times>
+    (('ctx, 'g) analysis_node \<times> analysis_edge_kind \<times>
+      ('ctx, 'g) analysis_node) list)"
+
+record ('ctx, 'g, 'a, 'd) analysis_graph_config =
+  local_of :: "'a \<Rightarrow> 'd"
+  route :: "pp \<Rightarrow> 'ctx \<Rightarrow> edge_action \<Rightarrow> 'd \<Rightarrow> 'ctx"
+  show_context :: "'ctx \<Rightarrow> string"
+  locals_for_pp :: "pp \<Rightarrow> vname list"
+  return_slot_for_pp :: "pp \<Rightarrow> vname option"
+  globals_to_show :: "vname list"
+  show_local :: "pp \<Rightarrow> 'ctx \<Rightarrow> vname list \<Rightarrow> 'd \<Rightarrow> string list"
+  format_return :: "pp \<Rightarrow> 'ctx \<Rightarrow> vname \<Rightarrow> 'd \<Rightarrow> string list"
+  show_global :: "'g \<Rightarrow> vname list \<Rightarrow> 'a \<Rightarrow> string list"
+  show_global_key :: "'g \<Rightarrow> string"
+  is_shared_global :: "'g \<Rightarrow> bool"
+  show_internal_globals :: bool
+  owner_of :: "pp \<Rightarrow> string"
+  cluster_label :: "string \<Rightarrow> 'ctx \<Rightarrow> string"
+
+fun graphviz_owner_of :: "graphviz_region list \<Rightarrow> pp \<Rightarrow> string" where
+  "graphviz_owner_of [] p = ''unknown''"
+| "graphviz_owner_of ((owner, ps) # regions) p =
+    (if mem_pp p ps then region_label owner else graphviz_owner_of regions p)"
+
+definition compiled_owner_of ::
+  "proc_table \<Rightarrow> pname list \<Rightarrow> com \<Rightarrow> pp \<Rightarrow> string" where
+  "compiled_owner_of \<Pi> ps main p =
+    graphviz_owner_of (compile_prog_regions \<Pi> ps main) p"
+
+definition cfg_point_list :: "cfg \<Rightarrow> pp list" where
+  "cfg_point_list g =
+    remdups (cfg_entry g # cfg_exit g #
+      (concat (map (\<lambda>e. case e of (u, a, v) \<Rightarrow> [u, v]) (cfg_edges_list g))
+       @ concat (map (\<lambda>c. case c of (call, ex, ret, dst) \<Rightarrow> [call, ex, ret])
+           (cfg_combines_list g))))"
+
+definition contextual_graph_domain ::
+  "cfg \<Rightarrow> (pp \<Rightarrow> 'ctx list) \<Rightarrow> ((pp \<times> 'ctx) + 'g) list" where
+  "contextual_graph_domain g contexts_for_pp =
+    concat (map (\<lambda>p. map (\<lambda>ctx. Inl (p, ctx)) (contexts_for_pp p))
+      (cfg_point_list g))"
+
+record procedure_scope =
+  scope_formals :: "vname list"
+  scope_locals :: "vname list"
+  scope_return_slot :: "vname option"
+
+fun graphviz_action_defs :: "edge_action \<Rightarrow> vname list" where
+  "graphviz_action_defs (EA_Assign x e) = [x]"
+| "graphviz_action_defs _ = []"
+
+definition owner_assigned_vars ::
+  "cfg \<Rightarrow> (pp \<Rightarrow> string) \<Rightarrow> string \<Rightarrow> vname list" where
+  "owner_assigned_vars g point_owner owner =
+    remdups (concat (map (\<lambda>e. case e of (u, a, v) \<Rightarrow>
+      if point_owner u = owner then graphviz_action_defs a else []) (cfg_edges_list g)))"
+
+definition compiled_procedure_scope ::
+  "proc_table \<Rightarrow> pname list \<Rightarrow> com \<Rightarrow> cfg \<Rightarrow> pp \<Rightarrow> procedure_scope" where
+  "compiled_procedure_scope \<Pi> ps main g p =
+    (let owner = compiled_owner_of \<Pi> ps main p;
+         decl = \<Pi> owner;
+         fs = if owner = ''main'' then [] else
+           (case decl of None \<Rightarrow> [] | Some d \<Rightarrow> formals d);
+         ret = if owner = ''main'' then None else
+           (case decl of None \<Rightarrow> None
+            | Some d \<Rightarrow> case result d of None \<Rightarrow> None | Some _ \<Rightarrow> Some ret_var);
+         ls = filter (\<lambda>x. x \<notin> set fs \<and> x \<noteq> ret_var)
+           (owner_assigned_vars g (compiled_owner_of \<Pi> ps main) owner)
+     in \<lparr>scope_formals = fs, scope_locals = ls, scope_return_slot = ret\<rparr>)"
+
+definition visible_global ::
+  "('ctx, 'g, 'a, 'd) analysis_graph_config \<Rightarrow> 'g \<Rightarrow> bool" where
+  "visible_global cfg k =
+    (is_shared_global cfg k \<or> show_internal_globals cfg)"
+
+definition covered_local_nodes ::
+  "(pp \<times> 'ctx) list \<Rightarrow> ('ctx, 'g) analysis_node list" where
+  "covered_local_nodes covered = map (\<lambda>pc. LocalNode (fst pc) (snd pc)) covered"
+
+fun local_node_member :: "(pp \<times> 'ctx) list \<Rightarrow> pp \<Rightarrow> 'ctx \<Rightarrow> bool" where
+  "local_node_member [] p ctx = False"
+| "local_node_member ((p', ctx') # covered) p ctx =
+    (if p = p' \<and> ctx = ctx' then True else local_node_member covered p ctx)"
+
+fun graph_node_member :: "('ctx, 'g) analysis_node list
+  \<Rightarrow> ('ctx, 'g) analysis_node \<Rightarrow> bool" where
+  "graph_node_member [] node = False"
+| "graph_node_member (node' # rest) node =
+    (if node = node' then True else graph_node_member rest node)"
+
+definition analysis_context_clusters ::
+  "('ctx, 'g, 'a, 'd) analysis_graph_config \<Rightarrow> (pp \<times> 'ctx) list
+    \<Rightarrow> ('ctx, 'g) analysis_cluster list" where
+  "analysis_context_clusters cfg covered =
+    remdups (map (\<lambda>pc. ContextCluster (owner_of cfg (fst pc)) (snd pc)) covered)"
+
+definition analysis_global_nodes ::
+  "('ctx, 'g, 'a, 'd) analysis_graph_config \<Rightarrow> 'g list
+    \<Rightarrow> ('ctx, 'g) analysis_node list" where
+  "analysis_global_nodes cfg keys =
+    map GlobalNode (filter (visible_global cfg) (remdups keys))"
+
+definition analysis_global_cluster ::
+  "('ctx, 'g) analysis_node list \<Rightarrow> ('ctx, 'g) analysis_cluster list" where
+  "analysis_global_cluster ns =
+    (if list_ex (\<lambda>n. case n of GlobalNode _ \<Rightarrow> True | _ \<Rightarrow> False) ns
+     then [GlobalCluster] else [])"
+
+definition analysis_intra_edges ::
+  "cfg \<Rightarrow> (pp \<times> 'ctx) list
+    \<Rightarrow> (('ctx, 'g) analysis_node \<times> analysis_edge_kind \<times>
+       ('ctx, 'g) analysis_node) list" where
+  "analysis_intra_edges g covered =
+    concat (map (\<lambda>src_ctx.
+      concat (map (\<lambda>e. case e of (u, a, v) \<Rightarrow>
+        if fst src_ctx = u \<and> \<not> is_enter_action a \<and>
+           local_node_member covered v (snd src_ctx)
+        then [(LocalNode u (snd src_ctx), IntraEdge a, LocalNode v (snd src_ctx))]
+        else []) (cfg_edges_list g))) covered)"
+
+definition analysis_enter_edges ::
+  "('ctx, 'g, 'a, 'd) analysis_graph_config \<Rightarrow> cfg \<Rightarrow> (pp \<times> 'ctx) list
+    \<Rightarrow> (pp \<times> 'ctx + 'g \<Rightarrow> 'a)
+    \<Rightarrow> (('ctx, 'g) analysis_node \<times> analysis_edge_kind \<times>
+       ('ctx, 'g) analysis_node) list" where
+  "analysis_enter_edges cfg g covered sol =
+    concat (map (\<lambda>src_ctx.
+      concat (map (\<lambda>e. case e of (u, a, v) \<Rightarrow>
+        if fst src_ctx = u \<and> is_enter_action a then
+          let callee_ctx = route cfg u (snd src_ctx) a
+              (local_of cfg (sol (Inl src_ctx)))
+          in if local_node_member covered v callee_ctx
+             then [(LocalNode u (snd src_ctx), EnterEdge a, LocalNode v callee_ctx)]
+             else []
+        else []) (cfg_edges_list g))) covered)"
+
+definition analysis_combine_edges ::
+  "('ctx, 'g, 'a, 'd) analysis_graph_config \<Rightarrow> cfg \<Rightarrow> (pp \<times> 'ctx) list
+    \<Rightarrow> (pp \<times> 'ctx + 'g \<Rightarrow> 'a)
+    \<Rightarrow> (('ctx, 'g) analysis_node \<times> analysis_edge_kind \<times>
+       ('ctx, 'g) analysis_node) list" where
+  "analysis_combine_edges cfg g covered sol =
+    concat (map (\<lambda>src_ctx.
+      concat (map (\<lambda>c. case c of (call, ex, ret, dst) \<Rightarrow>
+        if fst src_ctx = call then
+          concat (map (\<lambda>e. case e of (u, a, v) \<Rightarrow>
+            if u = call \<and> is_enter_action a then
+              let callee_ctx = route cfg call (snd src_ctx) a
+                  (local_of cfg (sol (Inl src_ctx)))
+              in if local_node_member covered ex callee_ctx \<and>
+                    local_node_member covered ret (snd src_ctx)
+                 then [(LocalNode ex callee_ctx,
+                       CombineEdge call dst (return_slot_for_pp cfg ex),
+                       LocalNode ret (snd src_ctx))]
+                 else []
+            else []) (cfg_edges_list g))
+        else []) (cfg_combines_list g))) covered)"
+
+fun analysis_local_domain :: "((pp \<times> 'ctx) + 'g) list \<Rightarrow> (pp \<times> 'ctx) list" where
+  "analysis_local_domain [] = []"
+| "analysis_local_domain (Inl pc # domain) = pc # analysis_local_domain domain"
+| "analysis_local_domain (Inr k # domain) = analysis_local_domain domain"
+
+fun analysis_global_domain :: "((pp \<times> 'ctx) + 'g) list \<Rightarrow> 'g list" where
+  "analysis_global_domain [] = []"
+| "analysis_global_domain (Inl pc # domain) = analysis_global_domain domain"
+| "analysis_global_domain (Inr k # domain) = k # analysis_global_domain domain"
+
+definition build_analysis_graph_parts ::
+  "('ctx, 'g, 'a, 'd) analysis_graph_config \<Rightarrow> cfg
+    \<Rightarrow> (pp \<times> 'ctx) list \<Rightarrow> 'g list \<Rightarrow> (pp \<times> 'ctx + 'g \<Rightarrow> 'a)
+    \<Rightarrow> ('ctx, 'g) analysis_graph" where
+  "build_analysis_graph_parts cfg g covered global_keys sol =
+    (let locals = covered_local_nodes covered;
+         globals = analysis_global_nodes cfg global_keys;
+         ns = locals @ globals
+     in (analysis_context_clusters cfg covered @ analysis_global_cluster ns,
+         ns,
+         analysis_intra_edges g covered @ analysis_enter_edges cfg g covered sol
+           @ analysis_combine_edges cfg g covered sol))"
+
+text \<open>The graph domain is an executable presentation choice.  Solver coverage remains
+  extensional and can be checked propositionally by clients.\<close>
+
+definition build_analysis_graph ::
+  "('ctx, 'g, 'a, 'd) analysis_graph_config \<Rightarrow> cfg
+    \<Rightarrow> ((pp \<times> 'ctx) + 'g) list \<Rightarrow> (pp \<times> 'ctx + 'g \<Rightarrow> 'a)
+    \<Rightarrow> ('ctx, 'g) analysis_graph" where
+  "build_analysis_graph cfg g domain sol =
+    build_analysis_graph_parts cfg g (analysis_local_domain (remdups domain))
+      (analysis_global_domain (remdups domain)) sol"
+
+definition analysis_graph_nodes ::
+  "('ctx, 'g) analysis_graph \<Rightarrow> ('ctx, 'g) analysis_node list" where
+  "analysis_graph_nodes graph = (case graph of (_, ns, _) \<Rightarrow> ns)"
+
+definition analysis_graph_edges ::
+  "('ctx, 'g) analysis_graph \<Rightarrow>
+    (('ctx, 'g) analysis_node \<times> analysis_edge_kind \<times> ('ctx, 'g) analysis_node) list" where
+  "analysis_graph_edges graph = (case graph of (_, _, es) \<Rightarrow> es)"
+
+definition analysis_graph_wf ::
+  "('ctx, 'g) analysis_graph \<Rightarrow> bool" where
+  "analysis_graph_wf graph =
+    (case graph of (clusters, ns, es) \<Rightarrow>
+      distinct clusters \<and>
+      distinct ns \<and>
+      distinct es \<and>
+      list_all (\<lambda>e. case e of (src, _, dst) \<Rightarrow> graph_node_member ns src \<and> graph_node_member ns dst) es)"
+
+fun analysis_node_position :: "('ctx, 'g) analysis_node list
+  \<Rightarrow> ('ctx, 'g) analysis_node \<Rightarrow> nat" where
+  "analysis_node_position [] n = 0"
+| "analysis_node_position (m # ms) n =
+    (if n = m then 0 else Suc (analysis_node_position ms n))"
+
+fun owner_contexts ::
+  "('ctx, 'g, 'a, 'd) analysis_graph_config \<Rightarrow> ('ctx, 'g) analysis_node list
+    \<Rightarrow> (string \<times> 'ctx) list" where
+  "owner_contexts cfg [] = []"
+| "owner_contexts cfg (LocalNode p ctx # ns) =
+    (owner_of cfg p, ctx) # owner_contexts cfg ns"
+| "owner_contexts cfg (GlobalNode k # ns) = owner_contexts cfg ns"
+
+fun context_position :: "'a list \<Rightarrow> 'a \<Rightarrow> nat" where
+  "context_position [] key = 0"
+| "context_position (key' # keys) key =
+    (if key = key' then 0 else Suc (context_position keys key))"
+
+definition analysis_node_id ::
+  "('ctx, 'g, 'a, 'd) analysis_graph_config \<Rightarrow> ('ctx, 'g) analysis_node list
+    \<Rightarrow> ('ctx, 'g) analysis_node \<Rightarrow> string" where
+  "analysis_node_id cfg ns n =
+    (case n of
+      LocalNode p ctx \<Rightarrow> owner_of cfg p @ ''_pp'' @ string_of_nat p @ ''_ctx''
+        @ string_of_nat (context_position (remdups (owner_contexts cfg ns))
+            (owner_of cfg p, ctx))
+    | GlobalNode k \<Rightarrow> ''global_'' @ string_of_nat (analysis_node_position ns n))"
+
+fun analysis_cluster_position :: "('ctx, 'g) analysis_cluster list
+  \<Rightarrow> ('ctx, 'g) analysis_cluster \<Rightarrow> nat" where
+  "analysis_cluster_position [] cluster = 0"
+| "analysis_cluster_position (cluster0 # clusters) cluster =
+    (if cluster0 = cluster then 0
+     else Suc (analysis_cluster_position clusters cluster))"
+
+definition analysis_cluster_id :: "('ctx, 'g) analysis_cluster list
+  \<Rightarrow> ('ctx, 'g) analysis_cluster \<Rightarrow> string" where
+  "analysis_cluster_id clusters cluster =
+    (case cluster of
+      GlobalCluster \<Rightarrow> ''cluster_globals''
+    | ContextCluster owner ctx \<Rightarrow> ''cluster_ctx_''
+        @ string_of_nat (analysis_cluster_position clusters cluster))"
+
+definition analysis_nodes_in_cluster ::
+  "('ctx, 'g, 'a, 'd) analysis_graph_config \<Rightarrow> ('ctx, 'g) analysis_cluster
+    \<Rightarrow> ('ctx, 'g) analysis_node list \<Rightarrow> ('ctx, 'g) analysis_node list" where
+  "analysis_nodes_in_cluster cfg cluster ns =
+    sort_key (\<lambda>n. case n of LocalNode p ctx \<Rightarrow> p | GlobalNode k \<Rightarrow> 0)
+      (filter (\<lambda>n. case (cluster, n) of
+        (ContextCluster owner ctx, LocalNode p ctx') \<Rightarrow> owner = owner_of cfg p \<and> ctx = ctx'
+      | (GlobalCluster, GlobalNode _) \<Rightarrow> True
+      | _ \<Rightarrow> False) ns)"
+
+definition graphviz_point_label :: "cfg \<Rightarrow> pp \<Rightarrow> string" where
+  "graphviz_point_label g p =
+    (if p = cfg_entry g \<or> mem_pp p (proc_entry_pps_list g) then ''start''
+     else if p = cfg_exit g \<or> mem_pp p (proc_exit_pps_list g) then ''end''
+     else ''pp'' @ string_of_nat p)"
+
+definition contextual_node_label ::
+  "('ctx, 'g, 'a, 'd) analysis_graph_config \<Rightarrow> cfg
+    \<Rightarrow> (pp \<times> 'ctx + 'g \<Rightarrow> 'a) \<Rightarrow> ('ctx, 'g) analysis_node \<Rightarrow> string" where
+  "contextual_node_label cfg g sol n =
+    (case n of
+      LocalNode p ctx \<Rightarrow> join_gv_nl
+        (graphviz_point_label g p #
+          show_local cfg p ctx (locals_for_pp cfg p)
+            (local_of cfg (sol (Inl (p, ctx))))
+          @ (case return_slot_for_pp cfg p of None \<Rightarrow> []
+             | Some ret \<Rightarrow> format_return cfg p ctx ret
+                 (local_of cfg (sol (Inl (p, ctx))))))
+    | GlobalNode k \<Rightarrow> join_gv_nl
+        (show_global_key cfg k # show_global cfg k (globals_to_show cfg) (sol (Inr k))))"
+
+definition analysis_node_attrs :: "cfg \<Rightarrow> ('ctx, 'g) analysis_node \<Rightarrow> string" where
+  "analysis_node_attrs g n =
+    (case n of
+      LocalNode p _ \<Rightarrow> ctx_debug_default_node_attrs g p
+    | GlobalNode _ \<Rightarrow> ''shape=note,width=2.2,fixedsize=false'')"
+
+fun enter_bindings :: "vname list \<Rightarrow> aexp list \<Rightarrow> string list" where
+  "enter_bindings [] _ = []"
+| "enter_bindings _ [] = []"
+| "enter_bindings (x # xs) (e # es) =
+    (x @ '' := '' @ string_of_aexp e) # enter_bindings xs es"
+
+definition enter_action_label :: "edge_action \<Rightarrow> string" where
+  "enter_action_label a =
+    (case a of EA_Enter xs es \<Rightarrow> ''enter'' @ gv_nl @ join_gv_nl (enter_bindings xs es)
+     | _ \<Rightarrow> string_of_action a)"
+
+definition source_action_label :: "edge_action \<Rightarrow> string" where
+  "source_action_label a =
+    (case a of EA_Assign x e \<Rightarrow>
+       if x = ret_var then ''ret := '' @ string_of_aexp e else string_of_action a
+     | _ \<Rightarrow> string_of_action a)"
+
+definition analysis_edge_attrs :: "analysis_edge_kind \<Rightarrow> string" where
+  "analysis_edge_attrs kind =
+    (case kind of
+      IntraEdge a \<Rightarrow> ''label='' @ dq @ source_action_label a @ dq
+    | EnterEdge a \<Rightarrow> ''color=purple,penwidth=2,label='' @ dq
+        @ enter_action_label a @ dq
+    | CombineEdge call dst ret \<Rightarrow> ''style=dashed,color=blue,label='' @ dq
+        @ (case (dst, ret) of
+             (Some x, Some r) \<Rightarrow> x @ '' := '' @ r
+           | (Some x, None) \<Rightarrow> ''return to '' @ x
+           | (None, _) \<Rightarrow> ''return / nop'')
+        @ dq
+    | GlobalReadEdge \<Rightarrow> ''style=dotted,color=gray,label='' @ dq @ ''read global'' @ dq
+    | GlobalWriteEdge \<Rightarrow> ''style=dotted,color=gray,label='' @ dq @ ''write global'' @ dq)"
+
+definition analysis_cluster_label ::
+  "('ctx, 'g, 'a, 'd) analysis_graph_config \<Rightarrow> ('ctx, 'g) analysis_cluster \<Rightarrow> string" where
+  "analysis_cluster_label cfg cluster =
+    (case cluster of
+      ContextCluster owner ctx \<Rightarrow> cluster_label cfg owner ctx
+    | GlobalCluster \<Rightarrow> ''Shared globals'')"
+
+fun analysis_order_pairs :: "'a list \<Rightarrow> ('a \<times> 'a) list" where
+  "analysis_order_pairs [] = []"
+| "analysis_order_pairs [x] = []"
+| "analysis_order_pairs (x # y # xs) = (x, y) # analysis_order_pairs (y # xs)"
+
+fun analysis_real_edge :: 
+  "(('ctx, 'g) analysis_node \<times> analysis_edge_kind \<times> ('ctx, 'g) analysis_node) list
+    \<Rightarrow> ('ctx, 'g) analysis_node \<Rightarrow> ('ctx, 'g) analysis_node \<Rightarrow> bool" where
+  "analysis_real_edge [] src dst = False"
+| "analysis_real_edge ((src', kind, dst') # es) src dst =
+    (if src = src' \<and> dst = dst' then True else analysis_real_edge es src dst)"
+
+definition analysis_ordering_dot ::
+  "('ctx, 'g, 'a, 'd) analysis_graph_config \<Rightarrow> ('ctx, 'g) analysis_node list
+    \<Rightarrow> (('ctx, 'g) analysis_node \<times> analysis_edge_kind \<times> ('ctx, 'g) analysis_node) list
+    \<Rightarrow> ('ctx, 'g) analysis_node list \<Rightarrow> string" where
+  "analysis_ordering_dot cfg ns es ordered =
+    concat (map (\<lambda>pair. case pair of (src, dst) \<Rightarrow>
+      ''    '' @ analysis_node_id cfg ns src @ '' -> '' @ analysis_node_id cfg ns dst
+      @ '' [style=invis,weight=10];'' @ nl)
+      (filter (\<lambda>pair. case pair of (src, dst) \<Rightarrow> \<not> analysis_real_edge es src dst)
+        (analysis_order_pairs ordered)))"
+
+definition analysis_cluster_dot ::
+  "('ctx, 'g, 'a, 'd) analysis_graph_config \<Rightarrow> cfg
+    \<Rightarrow> ('ctx, 'g) analysis_cluster list \<Rightarrow> ('ctx, 'g) analysis_node list
+    \<Rightarrow> (('ctx, 'g) analysis_node \<times> analysis_edge_kind \<times> ('ctx, 'g) analysis_node) list
+    \<Rightarrow> (pp \<times> 'ctx + 'g \<Rightarrow> 'a) \<Rightarrow> ('ctx, 'g) analysis_cluster \<Rightarrow> string" where
+  "analysis_cluster_dot cfg g clusters ns es sol cluster =
+    (let members = analysis_nodes_in_cluster cfg cluster ns
+     in ''  subgraph '' @ analysis_cluster_id clusters cluster @ '' {'' @ nl
+      @ ''    label='' @ dq @ analysis_cluster_label cfg cluster @ dq @ '';'' @ nl
+      @ ''    style=filled; color=lightgrey; fillcolor=white;'' @ nl
+      @ concat (map (\<lambda>n. ''    '' @ analysis_node_id cfg ns n @ '' [''
+          @ analysis_node_attrs g n @ '',label='' @ dq @ contextual_node_label cfg g sol n
+          @ dq @ ''];'' @ nl) members)
+      @ analysis_ordering_dot cfg ns es members
+      @ ''  }'' @ nl)"
+
+definition analysis_edge_dot ::
+  "('ctx, 'g, 'a, 'd) analysis_graph_config \<Rightarrow> ('ctx, 'g) analysis_node list
+    \<Rightarrow> (('ctx, 'g) analysis_node \<times> analysis_edge_kind \<times> ('ctx, 'g) analysis_node)
+    \<Rightarrow> string" where
+  "analysis_edge_dot cfg ns e =
+    (case e of (src, kind, dst) \<Rightarrow> ''  '' @ analysis_node_id cfg ns src @ '' -> ''
+      @ analysis_node_id cfg ns dst @ '' ['' @ analysis_edge_attrs kind @ ''];'' @ nl)"
+
+definition analysis_graph_to_dot ::
+  "('ctx, 'g, 'a, 'd) analysis_graph_config \<Rightarrow> cfg
+    \<Rightarrow> (pp \<times> 'ctx + 'g \<Rightarrow> 'a) \<Rightarrow> ('ctx, 'g) analysis_graph \<Rightarrow> string" where
+  "analysis_graph_to_dot cfg g sol graph =
+    (case graph of (clusters, ns, es) \<Rightarrow>
+      if analysis_graph_wf graph then
+        ''digraph AnalysisCFG {'' @ nl
+        @ ''  rankdir=TB;'' @ nl
+        @ ''  node [fontname='' @ dq @ ''Menlo'' @ dq @ ''];'' @ nl
+        @ concat (map (analysis_cluster_dot cfg g clusters ns es sol) clusters)
+        @ concat (map (analysis_edge_dot cfg ns) es)
+        @ ''}'' @ nl
+      else ''digraph AnalysisCFG { invalid_graph }'' @ nl)"
+
+definition contextual_analysis_dot ::
+  "('ctx, 'g, 'a, 'd) analysis_graph_config \<Rightarrow> cfg
+    \<Rightarrow> ((pp \<times> 'ctx) + 'g) list \<Rightarrow> (pp \<times> 'ctx + 'g \<Rightarrow> 'a) \<Rightarrow> string" where
+  "contextual_analysis_dot cfg g domain sol =
+    analysis_graph_to_dot cfg g sol (build_analysis_graph cfg g domain sol)"
+
 end
 
